Linglib.lean
@@ -116,6 +116,7 @@ import Linglib.Core.Data.List.TakeDrop
 import Linglib.Core.Data.Multiset.Antidiagonal
 import Linglib.Core.Data.Multiset.Powerset
 import Linglib.Core.Data.Multiset.Rel
+import Linglib.Core.Data.Option.Compatible
 import Linglib.Core.Data.Part
 import Linglib.Core.Data.RoseTree.Basic
 import Linglib.Core.Data.RoseTree.Count
